rupicola/io/IO.fst
@@ -63,15 +63,31 @@ let lem_theta_write (b:bool) (x:io_res OWrite b) (h:history) (lt:local_trace h) 
         (ensures wp2p (theta (write b)) h lt x) =
   assert (theta (write b) == (fun (h:history) (p:hist_post h (resexn unit)) -> (forall (lt:local_trace h) (r:resexn unit). lt == [EvWrite b r] ==> p (lt @ []) r))) by (assert (lt @ []) == lt; FStar.Tactics.compute ())
 
-(*//requires lt == []
-//ensures wp2p (theta (return x))
+let rec get_lt (h h':history) (lt:local_trace h) : Tot (local_trace h') (decreases lt) =
+  match lt with
+  | [] -> []
+  | ev :: tl -> begin
+    match ev with
+    | EvRead args res -> begin
+      // here we will need to check compatability of ev with h' and either return Inl or Inr of unit
+      assume (test_event h' ev); 
+      assume (well_formed_local_trace (ev::h) tl);
+      assume (forall (lt':local_trace (ev::h')). well_formed_local_trace h' (ev::lt')); 
+      ev :: (get_lt (ev::h) (ev::h') tl)
+      end
+    | EvWrite args res -> begin
+      // here we will need to check compatability of ev with h' and either return Inl or Inr of unit
+      assume (test_event h' ev); 
+      assume (well_formed_local_trace (ev::h) tl);
+      assume (forall (lt':local_trace (ev::h')). well_formed_local_trace h' (ev::lt'));
+      ev :: (get_lt (h++[ev]) (h'++[ev]) tl)
+      end
+    end
 
-assume val get_lt (h h':history) (lt:local_trace h) : (lt':local_trace h') // indution on lt
+let get_lt_correct (h h':history) (lt:local_trace h) :
+  Lemma ((lt == [] ==> (get_lt h h' []) == []) /\
+         (forall lt1 lt2. lt == (lt1 @ lt2) ==> (get_lt h h' (lt1 @ lt2)) == lt1 @ (get_lt (h++lt1) (h'++lt1) lt2))) = admit ()
 
-let hist_monotonic (wp:hist 'a) :
-Lemma (forall h h' (p':hist_post h' 'a). (wp h' p' ==> wp h (fun lt res -> p' (get_lt h h' lt) res))) = admit ()
-
-// equivalent up to renaming of local traces*)
 
 let rec theta_monotonic_hist (m:io 'a) :
 Lemma (forall h h' (p':hist_post h' 'a). (theta m h' p' ==> theta m h (fun lt res -> p' (get_lt h h' lt) res))) =
@@ -79,25 +95,95 @@ Lemma (forall h h' (p':hist_post h' 'a). (theta m h' p' ==> theta m h (fun lt re
   | Return x -> begin
     introduce forall h h' p'. theta m h' p' ==> theta m h (fun lt res -> p' (get_lt h h' lt) res) with begin
       introduce _ ==> _ with _. begin
-        let lt' : local_trace h' = [] in
-        let lt : local_trace h = [] in
-        assert (theta m h' p' == p' lt' x);
-        assert (theta m h (fun lt res -> p' (get_lt h h' lt) res) == (p' (get_lt h h' lt) x));
-        assume (p' lt' x ==> p' (get_lt h h' lt) x)
-        //assume (get_lt h h' lt == lt')
-        //admit ()
+        assert ((theta m h' p') == p' [] x);
+        assert ((theta m h (fun lt res -> p' (get_lt h h' lt) res)) == p' (get_lt h h' []) x);
+        get_lt_correct h h' []
       end
     end
     end
   | Call o args k -> begin
     introduce forall h h' p'. theta m h' p' ==> theta m h (fun lt res -> p' (get_lt h h' lt) res) with begin
+      introduce theta m h' p' ==> theta m h (fun lt res -> p' (get_lt h h' lt) res) with _. begin
+        assume ((theta m h' p') == (forall lt (r:io_res o args). lt == [op_to_ev o args r] ==> theta (k r) (h'++lt) (fun (lt':local_trace (h'++lt)) r -> p' (lt @ lt') r)));
+        assume ((theta m h (fun lt res -> p' (get_lt h h' lt) res)) == (forall lt (r:io_res o args). lt == [op_to_ev o args r] ==> theta (k r) (h++lt) (fun (lt':local_trace (h++lt)) r -> p' (get_lt h h' (lt @ lt')) r)));
+        introduce forall lt (r:io_res o args). lt == [op_to_ev o args r] ==> theta (k r) (h++lt) (fun (lt':local_trace (h++lt)) r -> p' (get_lt h h' (lt @ lt')) r) with begin
+          introduce lt == [op_to_ev o args r] ==> theta (k r) (h++lt) (fun (lt':local_trace (h++lt)) r -> p' (get_lt h h' (lt @ lt')) r) with _. begin
+            assert (theta (k r) (h'++lt) (fun (lt':local_trace (h'++lt)) r -> p' (lt @ lt') r));
+            theta_monotonic_hist (k r);
+            assert (forall h h' (p':hist_post h' 'a). (theta (k r) h' p' ==> theta (k r) h (fun lt res -> p' (get_lt h h' lt) res)));
+            eliminate forall h h' (p':hist_post h' 'a). (theta (k r) h' p' ==> theta (k r) h (fun lt res -> p' (get_lt h h' lt) res)) with (h++lt) (h'++lt) (fun (lt':local_trace (h'++lt)) r -> p' (lt @ lt') r);
+            assert (theta (k r) (h++lt) (fun lt_ res -> (fun (lt':local_trace (h'++lt)) r -> p' (lt @ lt') r) (get_lt (h++lt) (h'++lt) lt_) res));
+            assert (theta (k r) (h++lt) (fun lt_ res -> p' (lt @ (get_lt (h++lt) (h'++lt) lt_)) res));
+            introduce forall (lt':local_trace (h++lt)) r. (p' (get_lt h h' (lt @ lt')) r) ==  (p' (lt @ (get_lt (h++lt) (h'++lt) lt')) r) with begin
+              get_lt_correct h h' (lt @ lt')
+            end
+          end
+        end
+      end
+    end
+    end
+
+let theta_history_independence #a (m:io a) (h h':history) (lt:local_trace h) (fs_r:a) :
+  Lemma (requires wp2p (theta m) h lt fs_r)
+        (ensures wp2p (theta m) h' (get_lt h h' lt) fs_r) =
+  introduce forall (p':hist_post h' a). theta m h' p' ==> p' (get_lt h h' lt) fs_r with begin
+    introduce _ ==> _ with _. begin
+      theta_monotonic_hist m;
+      eliminate forall h h' p'. theta m h' p' ==> theta m h (fun lt res -> p' (get_lt h h' lt) res) with h h' p';
+      assert (forall (p:hist_post h a). theta m h p ==> p lt fs_r);
+      eliminate forall (p:hist_post h a). theta m h p ==> p lt fs_r with (fun lt res -> p' (get_lt h h' lt) res);
+      assert (p' (get_lt h h' lt) fs_r)
+    end
+  end
+
+(* DEFINITION UNFOLDING 
+assert (theta m h' p' == theta (Call o args k) h' p');
+        assert (theta m h (fun lt res -> p' (get_lt h h' lt) res) == theta (Call o args k) h (fun lt res -> p' (get_lt h h' lt) res));
+        assert (theta (Call o args k) h' p' == hist_bind (op_wp o args) (fun r -> theta (k r)) h' p') by (FStar.Tactics.compute ());
+        assert (theta (Call o args k) h (fun lt res -> p' (get_lt h h' lt) res) == hist_bind (op_wp o args) (fun r -> theta (k r)) h (fun lt res -> p' (get_lt h h' lt) res)) by (FStar.Tactics.compute ());
+        assert (hist_bind (op_wp o args) (fun r -> theta (k r)) h' p' == (op_wp o args) h' (hist_post_bind h' (fun r -> theta (k r)) p')) by (FStar.Tactics.compute ());
+        assert (hist_bind (op_wp o args) (fun r -> theta (k r)) h (fun lt res -> p' (get_lt h h' lt) res) == (op_wp o args) h (hist_post_bind h (fun r -> theta (k r)) (fun lt res -> p' (get_lt h h' lt) res))) by (FStar.Tactics.compute ());
+        assert ((op_wp o args) h' (hist_post_bind h' (fun r -> theta (k r)) p') == to_hist (fun h -> io_pre h o args) (fun h res lt -> io_post h o args res /\ lt == [op_to_ev o args res]) h' (hist_post_bind h' (fun r -> theta (k r)) p')) by (FStar.Tactics.compute ());
+        assert ((op_wp o args) h (hist_post_bind h (fun r -> theta (k r)) (fun lt res -> p' (get_lt h h' lt) res)) == to_hist (fun h -> io_pre h o args) (fun h res lt -> io_post h o args res /\ lt == [op_to_ev o args res]) h (hist_post_bind h (fun r -> theta (k r)) (fun lt res -> p' (get_lt h h' lt) res))) by (FStar.Tactics.compute ());
+        assert ((to_hist (fun h -> io_pre h o args) (fun h res lt -> io_post h o args res /\ lt == [op_to_ev o args res])) == (fun h p -> io_pre h o args /\ (forall (lt:local_trace h) (r:io_res o args). (io_post h o args r /\ lt == [op_to_ev o args r]) ==> p lt r))) by (FStar.Tactics.compute ());
+        assert ((to_hist (fun h -> io_pre h o args) (fun h res lt -> io_post h o args res /\ lt == [op_to_ev o args res]) h' (hist_post_bind h' (fun r -> theta (k r)) p')) == (fun h p -> io_pre h o args /\ (forall (lt:local_trace h) (r:io_res o args). (io_post h o args r /\ lt == [op_to_ev o args r]) ==> p lt r)) h' (hist_post_bind h' (fun r -> theta (k r)) p')) by (FStar.Tactics.compute ());
+        assert ((to_hist (fun h -> io_pre h o args) (fun h res lt -> io_post h o args res /\ lt == [op_to_ev o args res]) h (hist_post_bind h (fun r -> theta (k r)) (fun lt res -> p' (get_lt h h' lt) res))) == (fun h p -> io_pre h o args /\ (forall (lt:local_trace h) (r:io_res o args). (io_post h o args r /\ lt == [op_to_ev o args r]) ==> p lt r)) h (hist_post_bind h (fun r -> theta (k r)) (fun lt res -> p' (get_lt h h' lt) res))) by (FStar.Tactics.compute ());
+        assert ((fun h p -> io_pre h o args /\ (forall (lt:local_trace h) (r:io_res o args). (io_post h o args r /\ lt == [op_to_ev o args r]) ==> p lt r)) h' (hist_post_bind h' (fun r -> theta (k r)) p') == (io_pre h' o args /\ (forall lt (r:io_res o args). (io_post h' o args r /\ lt == [op_to_ev o args r]) ==> (hist_post_bind h' (fun r -> theta (k r)) p') lt r))) by (FStar.Tactics.compute ());
+        assert ((fun h p -> io_pre h o args /\ (forall (lt:local_trace h) (r:io_res o args). (io_post h o args r /\ lt == [op_to_ev o args r]) ==> p lt r)) h (hist_post_bind h (fun r -> theta (k r)) (fun lt res -> p' (get_lt h h' lt) res)) == (io_pre h o args /\ (forall lt (r:io_res o args). (io_post h o args r /\ lt == [op_to_ev o args r]) ==> (hist_post_bind h (fun r -> theta (k r)) (fun lt res -> p' (get_lt h h' lt) res)) lt r))) by (FStar.Tactics.compute ());
+        assert ((io_pre h o args /\ (forall lt (r:io_res o args). (io_post h o args r /\ lt == [op_to_ev o args r]) ==> (hist_post_bind h (fun r -> theta (k r)) (fun lt res -> p' (get_lt h h' lt) res)) lt r)) == (forall lt (r:io_res o args). lt == [op_to_ev o args r] ==> (hist_post_bind h (fun r -> theta (k r)) (fun lt res -> p' (get_lt h h' lt) res)) lt r)) by (FStar.Tactics.compute ());
+        assert ((io_pre h' o args /\ (forall lt (r:io_res o args). (io_post h' o args r /\ lt == [op_to_ev o args r]) ==> (hist_post_bind h' (fun r -> theta (k r)) p') lt r)) == (forall lt (r:io_res o args). lt == [op_to_ev o args r] ==> (hist_post_bind h' (fun r -> theta (k r)) p') lt r)) by (FStar.Tactics.compute ());
+        assert ((forall lt (r:io_res o args). lt == [op_to_ev o args r] ==> (hist_post_bind h' (fun r -> theta (k r)) p') lt r) == (forall lt (r:io_res o args). lt == [op_to_ev o args r] ==> theta (k r) (h'++lt) (hist_post_shift h' p' lt))) by (FStar.Tactics.compute ());
+        assert ((forall lt (r:io_res o args). lt == [op_to_ev o args r] ==> (hist_post_bind h (fun r -> theta (k r)) (fun lt res -> p' (get_lt h h' lt) res)) lt r) == (forall lt (r:io_res o args). lt == [op_to_ev o args r] ==> theta (k r) (h++lt) (hist_post_shift h (fun lt res -> p' (get_lt h h' lt) res) lt))) by (FStar.Tactics.compute ());
+        assert ((forall (lt:local_trace h'). (hist_post_shift h' p' lt) == (fun (lt':local_trace (h'++lt)) r -> p' (lt @ lt') r))) by (FStar.Tactics.compute ());
+        assert ((forall (lt:local_trace h). (hist_post_shift h (fun lt res -> p' (get_lt h h' lt) res) lt) == (fun (lt':local_trace (h++lt)) r -> (p' (get_lt h h' (lt @ lt')) r)))) by (FStar.Tactics.compute ());
+        assert ((forall lt (r:io_res o args). lt == [op_to_ev o args r] ==> theta (k r) (h'++lt) (hist_post_shift h' p' lt)) == (forall lt (r:io_res o args). lt == [op_to_ev o args r] ==> theta (k r) (h'++lt) (fun (lt':local_trace (h'++lt)) r -> p' (lt @ lt') r))) by (FStar.Tactics.compute ());
+        assert ((forall lt (r:io_res o args). lt == [op_to_ev o args r] ==> theta (k r) (h++lt) (hist_post_shift h (fun lt res -> p' (get_lt h h' lt) res) lt)) == (forall lt (r:io_res o args). lt == [op_to_ev o args r] ==> theta (k r) (h++lt) (fun (lt':local_trace (h++lt)) r -> (p' (get_lt h h' (lt @ lt')) r)))) by (FStar.Tactics.compute ());
+*)
+
+(*let rec theta_monotonic_hist' (m:io 'a) :
+Lemma (forall h h' (p':hist_post h' 'a). (theta m h' p' ==> theta m h (fun lt res -> p' (get_lt h h' lt) res))) =
+  match m with
+  | Return x -> () (*begin
+    introduce forall h h' p'. theta m h' p' ==> theta m h (fun lt res -> p' (get_lt h h' lt) res) with begin
+      introduce _ ==> _ with _. begin
+        assert (theta m h' p' == p' [] x);
+        assert (theta m h (fun lt res -> p' (get_lt h h' lt) res) == (p' [] x));
+        //assume (p' lt' x ==> p' (get_lt h h' lt) x)
+        //assume (get_lt h h' lt == lt')
+        admit ()
+      end
+    end
+    end*)
+  | _ -> admit ()
+  (*| Call o args k -> begin
+    introduce forall h h' p'. theta m h' p' ==> theta m h (fun lt res -> p' (get_lt h h' lt) res) with begin
       introduce _ ==> _ with _. begin
         assert (theta (Call o args k) == hist_bind (op_wp o args) (fun r -> theta (k r))) by (FStar.Tactics.compute ());
         assert (hist_bind (op_wp o args) (fun r -> theta (k r)) h' p' == (op_wp o args) h' (hist_post_bind h' (fun r -> theta (k r)) p')) by (FStar.Tactics.compute ());
-        assert ((op_wp o args) h' (hist_post_bind h' (fun r -> theta (k r)) p') == forall r. theta (k r) (h'++[op_to_ev o args r]) (fun lt' r -> p' ([op_to_ev o args r] @ lt') r)) by (FStar.Tactics.compute ());
-        introduce forall r. theta (k r) (h++[op_to_ev o args r]) (fun lt' r -> (p' (get_lt h h' ([op_to_ev o args r] @ lt')) r with begin
-          theta_monotonic_hist (k r);
-        end
+        //assert ((op_wp o args) h' (hist_post_bind h' (fun r -> theta (k r)) p') == forall r. theta (k r) (h'++[op_to_ev o args r]) (fun lt' r -> p' ([op_to_ev o args r] @ lt') r)) by (FStar.Tactics.compute ());
+        //introduce forall r. theta (k r) (h++[op_to_ev o args r]) (fun lt' r -> (p' (get_lt h h' ([op_to_ev o args r] @ lt')) r with begin
+        //  theta_monotonic_hist (k r);
+        //end
         //assume (forall r. theta (k r) (h++[op_to_ev o args r]) (fun lt' r -> (p' (get_lt h h' ([op_to_ev o args r] @ lt')) r));
         //assume ((op_wp o args) h (fun lt r -> theta (k r) (h++lt) (fun lt' r -> p' (get_lt h h' (lt @ lt')) r)))
         //assert (theta m h (fun lt res -> p' (get_lt h h' lt) res) == (p' (get_lt h h' lt) x));
@@ -106,12 +192,12 @@ Lemma (forall h h' (p':hist_post h' 'a). (theta m h' p' ==> theta m h (fun lt re
         admit ()
       end
     end
-    end
+  end*)
 
-let theta_history_independence #a (m:io a) (h h':history) (lt:local_trace h) (lt':local_trace h') (fs_r:a) :
+(*let theta_history_independence #a (m:io a) (h h':history) (lt:local_trace h) (lt':local_trace h') (fs_r:a) :
   Lemma (requires wp2p (theta m) h lt fs_r /\ lt == lt')
-        (ensures wp2p (theta m) h' (get_lt h h' lt) fs_r) =
-  match m with
+        (ensures wp2p (theta m) h' (get_lt h h' lt) fs_r) = admit ()*)
+  (*match m with
   | Return x -> begin
     assert (wp2p (theta m) h lt fs_r);
     assert (forall p. (theta m) h p ==> p [] x);
@@ -121,12 +207,13 @@ let theta_history_independence #a (m:io a) (h h':history) (lt:local_trace h) (lt
         let p : hist_post h a = fun lt res -> p' (get_lt h h' lt) res in
         eliminate forall p. (theta m) h p ==> p lt fs_r with p;
         assert ((theta m) h' p');
-        hist_wp_monotonic' (theta m);
+        theta_monotonic_hist m;
+        //hist_wp_monotonic' (theta m);
         assert (p lt fs_r);
         assert (p' (get_lt h h' lt) fs_r);
-        assert ((get_lt h h' lt) == lt')
+        //assert ((get_lt h h' lt) == lt');
   
-        //admit ()
+        admit ()
         //assert ((theta m) h p ==> p lt fs_r);
         //admit ()
       end
@@ -147,7 +234,7 @@ let theta_history_independence #a (m:io a) (h h':history) (lt:local_trace h) (lt
       assert ((theta m) h p ==> p lt fs_r);
       admit ()
     end
-  end*)
+  end*)*)
 
 
 
@@ -155,7 +242,7 @@ let theta_history_independence #a (m:io a) (h h':history) (lt:local_trace h) (lt
 
 
 
-let theta_history_independence' #a (m:io a) (h h':history) (lt:local_trace h) (lt':local_trace h') (fs_r:a) :
+(*let theta_history_independence' #a (m:io a) (h h':history) (lt:local_trace h) (fs_r:a) (st:steps e e' h lt) :
   Lemma (requires wp2p (theta m) h lt fs_r /\ lt == lt')
         (ensures wp2p (theta m) h' lt' fs_r) =
   match m with
@@ -188,5 +275,59 @@ let theta_history_independence' #a (m:io a) (h h':history) (lt:local_trace h) (l
       assert ((theta m) h p ==> p lt fs_r);
       admit ()
     end
+  end*)*)
+
+let theta_monotonic_hist'' #a #e #e' #h #lt (m:io a) (st:steps e e' h lt) :
+  Lemma (forall h h' (p':hist_post h' a). theta m h' p' ==> theta m h (fun lt res -> p' (construct_local_trace st h') res)) =
+  match m with
+  | Return x -> begin
+    introduce forall h h' p'. theta m h' p' ==> theta m h (fun lt res -> p' (construct_local_trace st h') res) with begin
+    introduce _ ==> _ with _. begin
+      assert (theta m h' p' == p' [] x);
+      assert (theta m h (fun lt res -> p' (construct_local_trace st h') res) == p' (construct_local_trace st h') x);
+      assume (p' [] x ==> p' (construct_local_trace st h') x)
+      end
+    end
+    end
+  | Call o args k -> begin
+    introduce forall h h' p'. theta m h' p' ==> theta m h (fun lt res -> p' (construct_local_trace st h') res) with begin
+    introduce theta m h' p' ==> theta m h (fun lt res -> p' (construct_local_trace st h') res) with _. begin
+      assert (theta (Call o args k) == hist_bind (op_wp o args) (fun r -> theta (k r))) by (FStar.Tactics.compute ());
+      assert (hist_bind (op_wp o args) (fun r -> theta (k r)) h' p' == (op_wp o args) h' (hist_post_bind h' (fun r -> theta (k r)) p')) by (FStar.Tactics.compute ());
+      assert ((op_wp o args) h' (hist_post_bind h' (fun r -> theta (k r)) p') == to_hist (fun h -> io_pre h o args) (fun h res lt -> io_post h o args res /\ lt == [op_to_ev o args res]) h' (hist_post_bind h' (fun r -> theta (k r)) p')) by (FStar.Tactics.compute ());
+      assert ((to_hist (fun h -> io_pre h o args) (fun h res lt -> io_post h o args res /\ lt == [op_to_ev o args res])) == (fun h p -> io_pre h o args /\ (forall (lt:local_trace h) (r:io_res o args). (io_post h o args r /\ lt == [op_to_ev o args r]) ==> p lt r))) by (FStar.Tactics.compute ());
+      assert ((to_hist (fun h -> io_pre h o args) (fun h res lt -> io_post h o args res /\ lt == [op_to_ev o args res]) h' (hist_post_bind h' (fun r -> theta (k r)) p')) == (fun h p -> io_pre h o args /\ (forall (lt:local_trace h) (r:io_res o args). (io_post h o args r /\ lt == [op_to_ev o args r]) ==> p lt r)) h' (hist_post_bind h' (fun r -> theta (k r)) p')) by (FStar.Tactics.compute ());
+      assert ((fun h p -> io_pre h o args /\ (forall (lt:local_trace h) (r:io_res o args). (io_post h o args r /\ lt == [op_to_ev o args r]) ==> p lt r)) h' (hist_post_bind h' (fun r -> theta (k r)) p') == (io_pre h' o args /\ (forall lt (r:io_res o args). (io_post h' o args r /\ lt == [op_to_ev o args r]) ==> (hist_post_bind h' (fun r -> theta (k r)) p') lt r))) by (FStar.Tactics.compute ());
+       assert ((io_pre h' o args /\ (forall lt (r:io_res o args). (io_post h' o args r /\ lt == [op_to_ev o args r]) ==> (hist_post_bind h' (fun r -> theta (k r)) p') lt r)) == (forall lt (r:io_res o args). lt == [op_to_ev o args r] ==> (hist_post_bind h' (fun r -> theta (k r)) p') lt r)) by (FStar.Tactics.compute ());
+       assert ((forall lt (r:io_res o args). lt == [op_to_ev o args r] ==> (hist_post_bind h' (fun r -> theta (k r)) p') lt r) == (forall lt (r:io_res o args). lt == [op_to_ev o args r] ==> theta (k r) (h'++lt) (hist_post_shift h' p' lt))) by (FStar.Tactics.compute ());
+       assert ((forall (lt:local_trace h'). (hist_post_shift h' p' lt) == (fun (lt':local_trace (h'++lt)) r -> p' (lt @ lt') r))) by (FStar.Tactics.compute ());
+       assert ((forall lt (r:io_res o args). lt == [op_to_ev o args r] ==> theta (k r) (h'++lt) (hist_post_shift h' p' lt)) == (forall lt (r:io_res o args). lt == [op_to_ev o args r] ==> theta (k r) (h'++lt) (fun (lt':local_trace (h'++lt)) r -> p' (lt @ lt') r))) by (FStar.Tactics.compute ());
+       assume ((theta m h' p') == (forall lt (r:io_res o args). lt == [op_to_ev o args r] ==> theta (k r) (h'++lt) (fun (lt':local_trace (h'++lt)) r -> p' (lt @ lt') r))); //by (FStar.Tactics.compute ());
+       assume ((theta m h (fun lt res -> p' (construct_local_trace st h') res)) == (forall lt (r:io_res o args). lt == [op_to_ev o args r] ==> theta (k r) (h++lt) (fun (lt':local_trace (h++lt)) r -> p' (construct_local_trace st h') r)));
+       introduce forall lt (r:io_res o args). lt == [op_to_ev o args r] ==> theta (k r) (h++lt) (fun (lt':local_trace (h++lt)) r -> p' (construct_local_trace st h') r) with begin
+         introduce _ ==> _ with _. begin
+           assert (lt == [op_to_ev o args r]);
+           let _ : io a = (k r) in
+           //let _ : steps e e' h lt = st in
+           //theta_monotonic_hist #a #e #e'
+           admit ()
+         end
+       end
+       //assert ((forall lt (r:io_res o args). lt == [op_to_ev o args r] ==> theta (k r) (h'++lt) (hist_post_shift h' p' lt)) == (forall lt (r:io_res o args). lt == [op_to_ev o args r] ==> theta (k r) (h'++lt) (fun lt' (r:io_res o args) -> p' (lt @ lt') r))) by (FStar.Tactics.compute ());
+      //admit ()
+    end
+    end
+    end
+
+let theta_history_independence' #a #e #e' (m:io a) (h h':history) (lt:local_trace h) (lt':local_trace h') (fs_r:a) (st':steps e e' h' lt') (st:steps e e' h lt) :
+  Lemma (requires wp2p (theta m) h (construct_local_trace st' h) fs_r)
+        (ensures wp2p (theta m) h' (construct_local_trace st h') fs_r) =
+  introduce forall (p':hist_post h' a). theta m h' p' ==> p' (construct_local_trace st h') fs_r with begin
+    introduce _ ==> _ with _. begin
+      theta_monotonic_hist m st;
+      eliminate forall h h' p'. theta m h' p' ==> theta m h (fun lt res -> p' (construct_local_trace st h') res) with h h' p';
+      assert (forall (p:hist_post h a). theta m h p ==> p (construct_local_trace st' h) fs_r);
+      eliminate forall (p:hist_post h a). theta m h p ==> p (construct_local_trace st' h) fs_r with (fun lt res -> p' (construct_local_trace st h') res);
+      assert (p' (construct_local_trace st h') fs_r)
+    end
   end*)
-  
